{
 "cells": [
  {
   "cell_type": "markdown",
   "metadata": {},
   "source": [
    "## Task 1\n",
    "\n",
    "Consider following system of differential equation $y' = Ay + f(t)$, \n",
    "where A - constant $3x3$ matrix, $y$, $f$ - 3-dimensional vectors:\n",
    "\n",
    "$$A = \\begin{pmatrix} 3, 1, 1, \\\\\n",
    "                  1, 0, -1, \\\\\n",
    "                  2, -1, 2 \\\\\n",
    "      \\end{pmatrix}, \n",
    "      f(t) = \\begin{pmatrix} 24 \\\\ -e^{2t} \\\\ 2e^{2t}\\\\ \\end{pmatrix}$$"
   ]
  },
  {
   "cell_type": "markdown",
   "metadata": {},
   "source": [
    "### Task 1.1 \n",
    "Solve homogeneous system of diff. eqs. $y' = Ay$ \n",
    "\n",
    "$$\\begin{vmatrix} 3 - \\lambda & 1 &         1 \\\\\n",
    "                  1 &           -\\lambda & -1 \\\\\n",
    "                  2 &           -1 &        2 - \\lambda\n",
    "  \\end{vmatrix} = 0; $$\n",
    "  \n",
    "$$ -8 - 2 \\lambda + 5 \\lambda^2 - \\lambda^3 = 0\\\\\n",
    "\\lambda_1 =  4, v_1 = \\begin{pmatrix} 1\\\\0\\\\1 \\end{pmatrix}\n",
    "\\lambda_2 =  2, v_2 = \\begin{pmatrix} -1\\\\-2\\\\3 \\end{pmatrix}\n",
    "\\lambda_3 = -1, v_3 = \\begin{pmatrix} -2\\\\5\\\\3  \\end{pmatrix} $$\n",
    "hence\n",
    "\n",
    "$$\\begin{pmatrix} \\dot{x}\\\\ \\dot{y} \\\\ \\dot{z} \\end{pmatrix} = \n",
    "   C_1e^{4t} \\begin{pmatrix} 1\\\\ 0 \\\\ 1 \\end{pmatrix} + \n",
    "   C_2e^{2t} \\begin{pmatrix} -1\\\\-2\\\\3 \\end{pmatrix} + \n",
    "   C_3e^{-t} \\begin{pmatrix} -2\\\\5\\\\3 \\end{pmatrix}$$"
   ]
  },
  {
   "cell_type": "markdown",
   "metadata": {},
   "source": [
    "### Task 1.2\n",
    "\n",
    "Calculate $e^{At}$, $det(e^{-A})$\n",
    "\n",
    "$$\\lambda_1 = 4, \\lambda_2 = 2, \\lambda_3 = -1 \\implies \\\\\n",
    "J_A = \\begin{pmatrix} 4 & 0 & 0 \\\\\n",
    "                      0 & 2 & 0 \\\\ \n",
    "                      0 & 0 & -1 \\\\\n",
    "      \\end{pmatrix}$$\n",
    "      \n",
    "$A = H^{-1} J_A H$\n",
    "where H - transition matrix to Jordan bases, hence\n",
    "$A H = J_A H$\n",
    "\n",
    "$$\\begin{pmatrix} \n",
    "      a_1 & a_2 & a_3 \\\\\n",
    "      b_1 & b_2 & b_3 \\\\\n",
    "      c_1 & c_2 & c_3\n",
    "  \\end{pmatrix}\n",
    "  \\begin{pmatrix}\n",
    "      3 & 1 & 1 \\\\ \n",
    "      1 & 0 & -1 \\\\ \n",
    "      2 & -1 & 2\n",
    "  \\end{pmatrix} = \n",
    "  \\begin{pmatrix}\n",
    "      4 & 0 & 0 \\\\ \n",
    "      0 & 2 & 0 \\\\\n",
    "      0 & 0 & -1\n",
    "  \\end{pmatrix}\n",
    "  \\begin{pmatrix}\n",
    "      a_1 & a_2 & a_3 \\\\\n",
    "      b_1 & b_2 & b_3 \\\\\n",
    "      c_1 & c_2 & c_3\n",
    "  \\end{pmatrix}\n",
    "  $$\n",
    "  \n",
    "$$\n",
    "  \\begin{cases}\n",
    "    3a_1 + a_2 +2a_3 &= 4a_1\\\\\n",
    "    a_1 - a_3 &= 4a_2\\\\\n",
    "    a_1 - a_2 + 2_a3 &= 4a_3\n",
    "  \\end{cases} \\implies a_1 = 7, a_2 = 1, a_3 = 3\\\\\n",
    "$$\n",
    "$$\n",
    "    \\begin{cases}\n",
    "    3b_1 + b_2 +2b_3 &= 2b_1\\\\\n",
    "    b_1 - b_3 &= 2b_2\\\\\n",
    "    b_1 - b_2 + 2_b3 &= 2b_3\\\\\n",
    "  \\end{cases} \\implies b_1 = 1, b_2 = 1, b_3 = -1\\\\\n",
    "$$\n",
    "$$\n",
    "  \\begin{cases}\n",
    "    3c_1 + c_2 +2c_3 &= -c_1\\\\\n",
    "    c_1 - c_3 &= -c_2\\\\\n",
    "    c_1 - c_2 + 2_c3 &= -c_3\\\\\n",
    "  \\end{cases} \\implies c_1 = 1, c_2 = -1, c_3 = 2\n",
    "$$\n",
    "In total:\n",
    "$$H = \\begin{pmatrix} 7 & 1 & 3 \\\\\n",
    "                      1 & 1 & -1 \\\\\n",
    "                      1 & -1 & 2\n",
    "      \\end{pmatrix}; \\\\\n",
    "  H^{-1} = 0.5 \\begin{pmatrix} -1 & 5 & 4 \\\\\n",
    "                                3 & -11 & 10 \\\\\n",
    "                                2 & -8 & -6\n",
    "           \\end{pmatrix}$$\n",
    "$$\\\\e^{At} = H^{-1} e^{J_A} H = \\begin{pmatrix}6 e^{-t} + 3 e^{2 t} - 7 e^{4 t} & -24 e^{-t} - 11 e^{2 t} + 35 e^{4 t} & -18 e^{-t} - 10 e^{2 t} + 28 e^{4 t}\\\\\n",
    "2 e^{-t} + 3 e^{2 t} - e^{4 t} & -8 e^{-t} - 11 e^{2 t} + 5 e^{4 t} & -6 e^{-t} - 10 e^{2 t} + 4 e^{4 t}\\\\\n",
    "4 e^{-t} - 3 e^{2 t} - e^{4 t} & -16 e^{-t} + 11 e^{2 t} + 5 e^{4 t} & -12 e^{-t} + 10 e^{2 t} + 4 e^{4 t}\\\\\n",
    "\\end{pmatrix}$$\n",
    "\n",
    "\n"
   ]
  },
  {
   "cell_type": "markdown",
   "metadata": {},
   "source": [
    "$$A = H^{-1}J_AH \\implies e^{-A} = -(H^{-1}e^{J_A}H) \\implies det(e^{-A}) = - det(H^{-1}) det(e^{J_A}) det(H) \\\\\n",
    "   det(e^{-A}) = -(-0.5) e^{5t} (-2) = -e^{5t}$$"
   ]
  },
  {
   "cell_type": "markdown",
   "metadata": {},
   "source": [
    "### Task 1.3\n",
    "\n",
    "Solve non-homogeneous diff. eq. using undefined coefficients method\n",
    "\n",
    "$f_1 = 24 = e^{\\sigma t}P_m(t) \\implies \\sigma = 0, m = 0, s = 0$\n",
    "$$\n",
    "    \\begin{cases}\n",
    "        x_{part, 1} &= A\\\\\n",
    "        y_{part, 1} &= B\\\\\n",
    "        z_{part, 1} &= C\\\\\n",
    "    \\end{cases}\n",
    "$$\n",
    "\n",
    "\n",
    "substituting into equation infer:\n",
    "\n",
    "\n",
    "$$\n",
    "    \\begin{cases}\n",
    "        3A + B + C + 24 &= 0 \\\\\n",
    "        A - C &= 0 \\\\\n",
    "        2A - B + 2C &= 0\\\\\n",
    "    \\end{cases} \\implies A = -3, B = 0, C = 3\n",
    "$$\n",
    "\n",
    "$f_2 = -e^{\\sigma 2t} \\implies \\sigma = 2, m = 0, s = 1$\n",
    "$$\n",
    "    \\begin{cases}\n",
    "        x_{part, 2} &= (A_1t + A_2)e^{2t}\\\\\n",
    "        y_{part, 2} &= (B_1t + B_2)e^{2t}\\\\\n",
    "        z_{part, 2} &= (C_1t + C_2)e^{2t}\\\\\n",
    "    \\end{cases}\n",
    "$$\n",
    "\n",
    "\n",
    "substituting into equation after canselling out all exponents we get:\n",
    "\n",
    "\n",
    "$$\n",
    "    \\begin{cases}\n",
    "        2A_1t + 2A_2 + A_1 = 3(A_1t + A_2) + (B_1t + B_2) + (C_1t + C_2)\\\\\n",
    "        2B_1t + 2B_2 + B_1 = (A_1t + A_2) - (C_1t + C_2) - 1\\\\\n",
    "        2C_1t + 2C_2 + C_1 = 2(A_1t + A_2) - (B_1t + B_2) + 2(C_1t + C_2) \\\\\n",
    "    \\end{cases} \\implies A_1 = 0, B_1 = 0, C_1 = 0, A_2 = 0, B_2 = -1, C_2 = 1;\n",
    "$$\n",
    "hence \n",
    "$$\n",
    "    \\begin{cases}\n",
    "        x_{part, 2} &= 0\\\\\n",
    "        y_{part, 2} &= -e^{2t}\\\\\n",
    "        z_{part, 2} &= e^{2t}\\\\\n",
    "    \\end{cases}\n",
    "$$\n",
    "\n",
    "$f_3 = 2e^{t} \\implies \\sigma = 2, m = 0, s = 1$\n",
    "$$\n",
    "    \\begin{cases}\n",
    "        x_{part, 3} &= (A_1t + A_2)e^{2t}\\\\\n",
    "        y_{part, 3} &= (B_1t + B_2)e^{2t}\\\\\n",
    "        z_{part, 3} &= (C_1t + C_2)e^{2t}\\\\\n",
    "    \\end{cases}\n",
    "$$\n",
    "substituting into equation after canselling out all exponents we get:\n",
    "\n",
    "\n",
    "$$\n",
    "    \\begin{cases}\n",
    "        2A_1t + 2A_2 + A_1 = 3(A_1t + A_2) + (B_1t + B_2) + (C_1t + C_2)\\\\\n",
    "        2B_1t + 2B_2 + B_1 = (A_1t + A_2) - (C_1t + C_2)\\\\\n",
    "        2C_1t + 2C_2 + C_1 = 2(A_1t + A_2) - (B_1t + B_2) + 2(C_1t + C_2) + 2\\\\\n",
    "    \\end{cases} \\implies A_1 = 0, B_1 = 0, C_1 = 0, A_2 = -\\frac{2}{3}, B_2 = -\\frac{-4}{3}, C_2 = 2;\n",
    "$$\n",
    "hence \n",
    "$$\n",
    "    \\begin{cases}\n",
    "        x_{part, 3} &= -\\frac{2}{3} e^{2t}\\\\\n",
    "        y_{part, 3} &= -\\frac{-4}{3}e^{2t}\\\\\n",
    "        z_{part, 3} &= 2e^{2t}\\\\\n",
    "    \\end{cases}\n",
    "$$\n",
    "\n",
    "totally:\n",
    "\n",
    "$$\n",
    "\\begin{cases}\n",
    "    x_{total} = C_1e^{4t} - C_2e^{2t} - 2e^{-t} - \\frac{2}{3}e^{2t} - 3\\\\\n",
    "    y_{total} = 2C_2e^{2t} + 5e^{-t} - e^{2t} - \\frac{4}{3}e^{2t}\\\\\n",
    "    z_{total} = -C_1e^{4t} + 3C_2e^{2t} + 3C_3e^{-t} + e^{2t} + 2e^{2t} + 3\n",
    "\\end{cases}\n",
    "$$"
   ]
  },
  {
   "cell_type": "markdown",
   "metadata": {},
   "source": [
    "## Task 2"
   ]
  },
  {
   "cell_type": "markdown",
   "metadata": {},
   "source": [
    "Solve given system of non-homogeneous differential equations using Lagrange's method\n",
    "\n",
    "$$\n",
    "\\begin{cases}\n",
    "    \\dot{x} = -4x + y -e^{-t}tg2t\\\\\n",
    "    \\dot{y} = -3x + 2y\n",
    "\\end{cases}\n",
    "$$\n",
    "\n",
    "corresponding homogeneous system:\n",
    "\n",
    "$$\n",
    "\\begin{cases}\n",
    "    \\dot{x} = -4x + y \\\\\n",
    "    \\dot{y} = -3x + 2y\n",
    "\\end{cases}; \\;\\;\\;\\;\n",
    "A = \\begin{pmatrix}\n",
    "        -4 & 1 \\\\\n",
    "        -3 & 2\n",
    "    \\end{pmatrix}; \\;\\;\\;\\; f_1 = -e^{-t}tg(2t), \\;\\;\\;\\; f_2 = 0;\n",
    "$$\n",
    "\n",
    "$$\n",
    "    \\lambda^{2} - 2\\lambda - 5 = 0 \\;\\;\\;\\; \\lambda_{1, 2} = -1 \\pm \\sqrt{6} \\;\\;\\;\\; v_{1, 2} = \n",
    "    \\begin{pmatrix} \\frac{1}{3} \\big( 3 \\pm \\sqrt{6} \\big) \\\\ 1 \\end{pmatrix}\n",
    "$$\n",
    "\n",
    "From this point I'd like to make expressions less obfuscated by making the following substitution: \n",
    "\n",
    "$$\n",
    "\\alpha_1 = \\frac{1}{3} \\big( 3 + \\sqrt{6} \\big)\\\\\n",
    "\\alpha_2 = \\frac{1}{3} \\big( 3 + \\sqrt{6} \\big)\n",
    "$$\n",
    "\n",
    "\n",
    "$$\n",
    "    \\begin{cases}\n",
    "        x = \\alpha_1 C_1e^{\\big(-1-\\sqrt{6}\\big)t} + \\alpha_2 C_2e^{\\big(-1 + \\sqrt{6}\\big)t}\\\\\n",
    "        y = C_1e^{\\big(-1-\\sqrt{6}\\big)t} + C_2e^{\\big(-1 + \\sqrt{6}\\big)t}\n",
    "    \\end{cases}\n",
    "$$\n",
    "\n",
    "Applying Lagranges method we get the following:\n",
    "$$\n",
    "\\begin{cases}\n",
    "    \\alpha_1 C^{'}_1e^{\\big(-1-\\sqrt{6}\\big)t} + \\alpha_2 C^{'}_2e^{\\big(-1 + \\sqrt{6}\\big)t} = -e^{-t}tg(2t)\\\\\n",
    "    C^{'}_1e^{\\big(-1-\\sqrt{6}\\big)t} + C^{'}_2e^{\\big(-1 + \\sqrt{6}\\big)t} = 0\n",
    "\\end{cases}\n",
    "$$\n",
    "\n",
    "$$\n",
    "    C^{'}_{2} = \\frac{e^{-t}tg(2t)}{{e^{\\big(-1 + \\sqrt{6}\\big)t}\\big(\\alpha_2 - \\alpha_1\\big)}}\\\\\n",
    "    C^{'}_{1} = -e^{2\\sqrt{6}t}\\frac{e^{-t}tg(2t)}{{e^{\\big(-1 + \\sqrt{6}\\big)t}\\big(\\alpha_2 - \\alpha_1\\big)}}\n",
    "$$\n",
    "\n",
    "$$\n",
    "    C_{1} = \\int{\\bigg(-e^{2\\sqrt{6}t}\\frac{e^{-t}tg(2t)}{{e^{\\big(-1 + \\sqrt{6}\\big)t}\\big(\\alpha_2 - \\alpha_1\\big)}}\\bigg)dt} + \\tilde{C_1}\\\\\n",
    "    C_{2} = \\int{\\bigg( \\frac{e^{-t}tg(2t)}{{e^{\\big(-1 + \\sqrt{6}\\big)t}\\big(\\alpha_2 - \\alpha_1\\big)}}\\bigg)dt} + \\tilde{C_2}\n",
    "$$\n",
    "\n",
    "totally:\n",
    "\n",
    "$$\n",
    "    \\begin{cases}\n",
    "        x = \\alpha_1 \\int{\\bigg(-e^{2\\sqrt{6}t}\\frac{e^{-t}tg(2t)}{{e^{\\big(-1 + \\sqrt{6}\\big)t}\\big(\\alpha_2 - \\alpha_1\\big)}}\\bigg)dt} + \\tilde{C_1}e^{\\big(-1-\\sqrt{6}\\big)t} + \\alpha_2 C_{2} = \\int{\\bigg( \\frac{e^{-t}tg(2t)}{{e^{\\big(-1 + \\sqrt{6}\\big)t}\\big(\\alpha_2 - \\alpha_1\\big)}}\\bigg)dt} + \\tilde{C_2}e^{\\big(-1 + \\sqrt{6}\\big)t}\\\\\n",
    "        y = \\int{\\bigg(-e^{2\\sqrt{6}t}\\frac{e^{-t}tg(2t)}{{e^{\\big(-1 + \\sqrt{6}\\big)t}\\big(\\alpha_2 - \\alpha_1\\big)}}\\bigg)dt} + \\tilde{C_1}e^{\\big(-1-\\sqrt{6}\\big)t} + C_{2} = \\int{\\bigg( \\frac{e^{-t}tg(2t)}{{e^{\\big(-1 + \\sqrt{6}\\big)t}\\big(\\alpha_2 - \\alpha_1\\big)}}\\bigg)dt} + \\tilde{C_2}e^{\\big(-1 + \\sqrt{6}\\big)t}\n",
    "    \\end{cases}\n",
    "$$\n",
    "\n",
    "app"
   ]
  },
  {
   "cell_type": "markdown",
   "metadata": {},
   "source": []
  },
  {
   "cell_type": "code",
   "execution_count": null,
   "metadata": {},
   "outputs": [],
   "source": []
  },
  {
   "cell_type": "code",
   "execution_count": null,
   "metadata": {},
   "outputs": [],
   "source": []
  }
 ],
 "metadata": {
  "kernelspec": {
   "display_name": "Python 3",
   "language": "python",
   "name": "python3"
  },
  "language_info": {
   "codemirror_mode": {
    "name": "ipython",
    "version": 3
   },
   "file_extension": ".py",
   "mimetype": "text/x-python",
   "name": "python",
   "nbconvert_exporter": "python",
   "pygments_lexer": "ipython3",
   "version": "3.7.2"
  }
 },
 "nbformat": 4,
 "nbformat_minor": 2
}
